TODO linearsearch, TOFIX mergesortarray

verification/LinearSearch.dfy
@@ -15,3 +15,104 @@ ensures i == -1 ==> forall j:: 0 <= j < a.Length ==> a[j] != key
     i := -1;
   }
 }
+
+// Checks if key is in array
+predicate InsideArray(a:array<int>, key:int)
+reads a 
+{
+  exists i:nat :: i<a.Length && a[i] == key
+}
+
+predicate InsideUpTo(a:array<int>, key:int, high:nat)
+requires high <= a.Length
+reads a
+{
+  exists i:nat :: i<high && a[i] == key
+}
+
+// Returns number of matches of key in sequence
+function Matches(s:seq<int>, key:int) : nat
+decreases s 
+{
+  if (|s| == 0) then 0
+  else if (s[0] == key) then 1 + Matches(s[1..], key)
+  else Matches(s[1..], key)
+}
+
+// Similar to above but as a method checking an array, low is the index to start checking from
+method ArrayMatches(a:array<int>, key:int, low:nat) returns (matches:nat)
+decreases a.Length - low
+ensures low < a.Length ==> matches == Matches(a[low..], key)
+ensures low >= a.Length ==> matches == 0
+requires a != null
+{
+  if (low >= a.Length){
+    matches := 0;
+  } else if (a[low] == key){
+    matches := ArrayMatches(a, key, low+1);
+    matches := matches + 1;
+  } else {
+    matches := ArrayMatches(a, key, low+1);
+  }
+}
+
+method LinearSearchMultiple(a:array<int>, key:int) returns (r:array<int>)
+requires a != null
+ensures forall i:nat :: i< r.Length ==> r[i] == key
+ensures r.Length == 0 ==> Matches(a[..],key) == 0
+ensures r.Length != 0 ==> forall i:nat :: i<a.Length ==> (InsideUpTo(r, a[i], r.Length) <==> a[i] == key) 
+ensures r.Length != 0 ==> multiset(r[..]) <= multiset(a[..]) 
+ensures r.Length != 0 ==> !(multiset(r[..] + [key]) <= multiset(a[..]))
+{
+  // Find number of matches to init returned array with appropriate size
+  var matches := ArrayMatches(a, key, 0);
+  assert matches == Matches(a[..], key);
+  r := new int[matches];
+  // If no matches leave early
+  if (r.Length == 0){
+    return;
+  }
+
+  var i := 0;
+  var j := 0;
+  assert forall k:nat :: k<i<a.Length ==> (InsideUpTo(r, a[k], r.Length) <==> a[k] == key);
+  assert matches == r.Length;
+  assert Matches(a[i..], key) == matches;
+  assert Matches(a[i..], key) == r.Length;
+  assert multiset(r[..j]) <= multiset(a[..]);
+
+  while (i < a.Length || j < r.Length)
+  decreases a.Length + matches -i -j
+  invariant 0 <= i <= a.Length
+  invariant forall k:nat :: k<j<=r.Length ==> r[k] == key
+  invariant j <= matches && j <= r.Length
+  invariant r.Length - j == Matches(a[i..], key);
+  invariant forall k:nat :: k<i<=a.Length ==> (InsideUpTo(r, a[k], j) <==> a[k] == key)
+  invariant multiset(r[..j]) <= multiset(a[..])
+  {
+    if (a[i] == key){
+      r[j] := a[i];
+      assert a[i] == key;
+      assert multiset(r[..j]) <= multiset(a[..]);
+      assert InsideArray(a, r[j]);
+      //assert multiset([r[j]]) <= multiset(a[..]);
+      //assert multiset(r[..j]+[r[j]]) <= multiset(a[..]);
+      j := j + 1;
+      //assert multiset(r[..j-1]) <= multiset(a[..]);
+      var gho := r[..j-1]+[r[j-1]];
+      //assert Matches(gho[..], key) <= Matches(a[..], key);
+      //assert multiset(gho) <= multiset(a[..]);
+      //assert multiset(r[..j]) <= multiset(a[..]);
+      
+    }
+    //assert multiset(r[..j]) <= multiset(a[..]);
+    //assert multiset([r[j]]) <= multiset(a[..]);
+    i := i + 1;
+  }
+  assert i == a.Length;
+  assert forall k:nat :: k<i<=a.Length ==> (InsideUpTo(r, a[k], j) <==> a[k] == key);
+  assert forall k:nat :: k<a.Length ==> (InsideUpTo(r, a[k], j) <==> a[k] == key);
+  assert j == r.Length;
+  assert InsideUpTo(r, key, r.Length) <==> InsideArray(r, key);
+  
+}
