verification/MergeSort.dfy
@@ -93,95 +93,6 @@ ensures s == [i] + r
 }
 
 
-// Merges 2 adjacent sub arrays within an array
-// low, mid and high are the indcies for these arrays
-method MergeSubarrays(a:array<int>, low:nat, mid:nat, high:nat)
-modifies a
-requires a != null
-requires low<mid<high<=a.Length
-requires InOrder(a[low..mid]) && InOrder(a[mid..high])
-ensures multiset(a[low..high]) == multiset(old(a[low..high]))
-ensures InOrder(a[low..high])
-ensures old(a[..low]) == a[..low] && old(a[high..]) == a[high..];
-ensures multiset(a[..]) == multiset(old(a[..]))
-{
-	var m := Merge(a[low..mid], a[mid..high]);
-
-	assert a[low..mid]+a[mid..high] == a[low..high]; 
-	assert |m| == high-low;
-
-	var high : nat := |m|+low;
-	CopyIntoArray(m, a, low);
-
-	assert m == a[low..high];
-	assert a[..] == a[..low]+a[low..high]+a[high..];
-	assert old(a[..] == a[..low]+a[low..high]+a[high..]);
-}
-
-// Sorts given array within indices low to high
-// Open at low, closed at high
-method MergeSortArray(a:array<int>, low:nat, high:nat)
-decreases a, high - low
-modifies a
-requires a != null
-requires a.Length >= 0
-requires low<=high<=a.Length
-ensures multiset(old(a[low..high])) == multiset(a[low..high])
-ensures a[..low] == old(a[..low]) && a[high..] == old(a[high..])
-ensures multiset(a[..]) == multiset(old(a[..]))
-ensures InOrder(a[low..high])
-{
-	var mid:nat := low + (high-low)/2;	// finding midpoint in subsection of array
-	// If array is more than one value, sort
-	if (a.Length > 1 && low < mid)
-	{
-		MergeSortArray(a, low, mid);	// Recursively sort left array
-		assert old(a[mid..high]) == a[mid..high];
-
-		MergeSortArray(a, mid, high);	// Recursively sort right array
-		assert old(a[low..mid]+a[mid..high] == a[low..high]);
-		assert a[low..mid]+a[mid..high] == a[low..high];	// Remind dafny something super obvious
-
-		MergeSubarrays(a, low, mid, high);	// Merging left and right
-	} // Else no need to sort array
-}
-
-// Copies a given sequence into an array, at a given starting index low
-method CopyIntoArray(s:seq<int>, a:array<int>, low:nat)
-modifies a
-requires a != null
-requires |s| > 0
-requires |s| <= a.Length - low;
-ensures forall i :: 0<=i<|s| ==> (s[i] == a[i+low])
-ensures old(a[..low]) == a[..low] && old(a[|s|+low..]) == a[|s|+low..]
-{
-	// Simple loop that seq into array
-	var i := 0;
-	while (i < |s|)
-	decreases |s| - i
-	invariant i <= |s|
-	invariant forall j :: 0<=j<i ==> s[j] == a[low+j]
-	invariant old(a[..low]) == a[..low] && old(a[|s|+low..]) == a[|s|+low..]
-	{
-		a[low+i] := s[i];
-		i := i + 1;
-	}
-}
-
-// Super simple print array
-method printArray(a:array)
-requires a != null
-{
-	var i := 0;
-	while (i < a.Length)
-	decreases a.Length - i
-	{
-		print a[i], " ";
-		i := i + 1;
-	}
-	print '\n';
-}
-
 // Real simple tests
 method Main(){
 	// Testing with sequences
@@ -200,21 +111,21 @@ method Main(){
 	assert (r == c);
 	print r, '\n';
 
-	var d := new int[5];
-	d[0], d[1], d[2], d[3], d[4] := 9, 4, 6, 3, 8;
-	assert d[0]==9 && d[1]==4 && d[2]==6 && d[3]==3 && d[4]==8;
-	MergeSortArray(d, 0, 5);
-	printArray(d);
-	// NOTE: below asserts commented out as they change verification time from 5 sec to 30 sec
-	//assert InOrder(d[0..5]);
+	// var d := new int[5];
+	// d[0], d[1], d[2], d[3], d[4] := 9, 4, 6, 3, 8;
+	// assert d[0]==9 && d[1]==4 && d[2]==6 && d[3]==3 && d[4]==8;
+	// MergeSortArray(d, 0, 5);
+	// printArray(d);
+	// // NOTE: below asserts commented out as they change verification time from 5 sec to 30 sec
+	// //assert InOrder(d[0..5]);
 
-	var e := new int[0];
-	MergeSortArray(e, 0, 0);
-	//assert InOrder(e[..]);
+	// var e := new int[0];
+	// MergeSortArray(e, 0, 0);
+	// //assert InOrder(e[..]);
 
-	var f := new int[5];
-	CopyIntoArray(c, f, 0);
-	MergeSortArray(f, 0, f.Length);
-	printArray(f);
+	// var f := new int[5];
+	// CopyIntoArray(c, f, 0);
+	// MergeSortArray(f, 0, f.Length);
+	// printArray(f);
 	//assert InOrder(f[..]);
 }
