verification/MergeSortArray.dfy
@@ -1,0 +1,146 @@
+// Super simple print array
+method printArray(a:array)
+requires a != null
+{
+	var i := 0;
+	while (i < a.Length)
+	decreases a.Length - i
+	{
+		print a[i], " ";
+		i := i + 1;
+	}
+	print '\n';
+}
+
+// Copies a given sequence into an array, at a given starting index low
+method CopyIntoArray(s:seq<int>, a:array<int>, low:nat)
+modifies a
+requires a != null
+requires |s| > 0
+requires |s| <= a.Length - low;
+ensures forall i :: 0<=i<|s| ==> (s[i] == a[i+low])
+ensures old(a[..low]) == a[..low] && old(a[|s|+low..]) == a[|s|+low..]
+{
+	// Simple loop that seq into array
+	var i := 0;
+	while (i < |s|)
+	decreases |s| - i
+	invariant i <= |s|
+	invariant forall j :: 0<=j<i ==> s[j] == a[low+j]
+	invariant old(a[..low]) == a[..low] && old(a[|s|+low..]) == a[|s|+low..]
+	{
+		a[low+i] := s[i];
+		i := i + 1;
+	}
+}
+
+// Checks that sequence is ordered
+predicate InOrder(a:seq<int>)
+{
+	forall i, j :: 0 <= i < j < |a| ==> a[i] <= a[j]
+}
+
+// Checks that every element in a are less than or equal to every element in b
+predicate lessThanEqualSeq(a:seq<int>, b:seq<int>){
+	forall i, j :: 0<=i<|a| && 0<=j<|b| ==> a[i] <= b[j]
+}
+
+// Sorts given array within indices low to high
+// Open at low, closed at high
+// method MergeSortArray(a:array<int>, low:nat, high:nat)
+// decreases a, high - low
+// modifies a
+// requires a != null
+// requires a.Length >= 0
+// requires low<=high<=a.Length
+// ensures multiset(old(a[low..high])) == multiset(a[low..high])
+// ensures a[..low] == old(a[..low]) && a[high..] == old(a[high..])
+// ensures multiset(a[..]) == multiset(old(a[..]))
+// ensures InOrder(a[low..high])
+// {
+// 	var mid:nat := low + (high-low)/2;	// finding midpoint in subsection of array
+// 	// If array is more than one value, sort
+// 	if (a.Length > 1 && low < mid)
+// 	{
+// 		MergeSortArray(a, low, mid);	// Recursively sort left array
+// 		assert old(a[mid..high]) == a[mid..high];
+
+// 		MergeSortArray(a, mid, high);	// Recursively sort right array
+// 		assert old(a[low..mid]+a[mid..high] == a[low..high]);
+// 		assert a[low..mid]+a[mid..high] == a[low..high];	// Remind dafny something super obvious
+
+// 		MergeSubarrays(a, low, mid, high);	// Merging left and right
+// 	} // Else no need to sort array
+// }
+
+// Merges 2 adjacent sub arrays within an array
+// low, mid and high are the indcies for these arrays
+method MergeSubarrays(a:array<int>, low:nat, mid:nat, high:nat)
+modifies a
+requires a != null
+requires low<mid<high<=a.Length
+requires InOrder(a[low..mid]) && InOrder(a[mid..high])
+ensures multiset(a[low..high]) == multiset(old(a[low..high]))
+ensures InOrder(a[low..high])
+ensures old(a[..low]) == a[..low] && old(a[high..]) == a[high..];
+ensures multiset(a[..]) == multiset(old(a[..]))
+{
+	assert a[..low] == old(a[..low]);
+	// Creating temp arrays for left and right
+	var i, j := 0,0;
+	var left, right := new int[mid-low], new int[high-mid];
+	assert left.Length +  right.Length == high-low;
+	while (i < mid-low)
+	decreases mid-low -i
+	invariant a[..] == old(a[..])
+	invariant i <= mid-low
+	invariant left[..i] == a[low..low+i]
+	{
+		left[i] := a[low+i];
+		i := i + 1;
+	}
+	while (j < high-mid) 
+
+	decreases high-mid -j
+	invariant a[..] == old(a[..])
+	invariant j <= high-mid
+	invariant right[..j] == a[mid..mid+j]
+	{
+		right[j] := a[mid+j];
+		j := j + 1;
+	}
+	assert a[..low] == old(a[..low]);
+
+	assert InOrder(left[..]) && InOrder(right[..]);
+	// Merge temp arrays back into a[low..high]
+	i,j := 0,0;
+	var k := low;
+	assert mid-low == left.Length && high-mid == right.Length;
+	while (i < left.Length && j < right.Length)
+	decreases left.Length + right.Length - i - j
+	invariant k <= a.Length && k >= low
+	invariant i <= left.Length && j <= right.Length
+	invariant InOrder(a[low..k]) && InOrder(left[i..]) && InOrder(right[j..])
+	invariant a[..low] == old(a[..low])
+	invariant multiset(a[low..k]) == multiset(left[..i] + right[..j])
+	{
+		if (left[i] <= right[j]){
+			assert multiset(a[low..k]) == multiset(left[..i] + right[..j]);
+			assert a[k] <= left[i];
+			a[k] := left[i];
+			k := k + 1;
+			i := i + 1;
+			assert multiset(a[low..k]) == multiset(left[..i] + right[..j]);
+		} else {
+			assert multiset(a[low..k]) == multiset(left[..i] + right[..j]);
+			assert a[k] <= right[j];
+			a[k] := right[j];
+			k := k + 1;
+			j := j + 1;
+			assert multiset(a[low..k]) == multiset(left[..i] + right[..j]);
+		}
+		assert multiset(a[low..k]) == multiset(left[..i] + right[..j]);
+	}
+
+
+}
